Pointer Logic (#32)
* pointer stuff

* clean up

* ltac fun

* pointer arithmetic

* value and pointer type

* concrete

* init/uninit and illegal accesses

* SMT representation for memory programs.

* clean up

* SMT representation for memory programs

* interpret symbolic

* discharge mem expr to z3 v1

* Added bounds checks + better discharge to Z3.

* extended lemmas

* fix dune script

* ite instead of max

* adjust internal int representation and clean up inefficient concrete/symbolic lemma

* modularized large functions and lemmas

* extended testing

* changes for copilot review

* test framework adjustment

* added some docs to readme

* a couple ops

* conditionals

* more changes from copilot review

* Fix scalar suffix handling in /MemSolver.ml

Co-authored-by: Copilot <175728472+Copilot@users.noreply.github.com>

* improved naming schema for rocq representation of Z3 query and extended mem IR bit operations

* annotated tests

* minor test update

---------

Co-authored-by: Lander Duncan <134824437+LanderDuncan@users.noreply.github.com>
Co-authored-by: Anirudh Sivaraman <sk.anirudh@gmail.com>
Co-authored-by: Copilot <175728472+Copilot@users.noreply.github.com>

extracted_code/CrTypeIF.ml
@@ -1,0 +1,96 @@
+module BinNums = struct
+  include BinNums
+  type positive = [%import: BinNums.positive]
+  [@@deriving sexp]
+  type coq_Z = [%import: BinNums.coq_Z]
+  [@@deriving sexp]
+end
+module Datatypes = struct
+  include Datatypes
+  type ('a, 'b) prod = [%import: ('a, 'b) Datatypes.prod]
+  [@@deriving sexp]
+  type 'a list = [%import: 'a Datatypes.list]
+  [@@deriving sexp]
+end
+module Integers = struct
+  include Integers
+  type bit_int = [%import: Integers.bit_int]
+  [@@deriving sexp]
+end
+module MyInts = struct
+  include MyInts
+  type uint8 = [%import: MyInts.uint8]
+  [@@deriving sexp]
+  type uint16 = [%import: MyInts.uint16]
+  [@@deriving sexp]
+  type uint32 = [%import: MyInts.uint32]
+  [@@deriving sexp]
+  type uint64 = [%import: MyInts.uint64]
+  [@@deriving sexp]
+  type uintbptr = [%import: MyInts.uintbptr]
+  [@@deriving sexp]
+end
+module CrVal = struct
+include CrVal
+type coq_CrInt_T = [%import: CrVal.coq_CrInt_T]
+[@@deriving sexp]
+type coq_CrPtr_T = [%import: CrVal.coq_CrPtr_T]
+[@@deriving sexp]
+type coq_CrVal = [%import: CrVal.coq_CrVal]
+[@@deriving sexp]
+end
+module CrIdentifiers = struct
+  include CrIdentifiers
+  type coq_Header = [%import: CrIdentifiers.coq_Header]
+  [@@deriving sexp]
+  type coq_State = [%import: CrIdentifiers.coq_State]
+  [@@deriving sexp]
+  type coq_Ctrl = [%import: CrIdentifiers.coq_Ctrl]
+  [@@deriving sexp]
+end
+module CrTransformer = struct
+  include CrTransformer
+  type coq_FunctionArgument = [%import: CrTransformer.coq_FunctionArgument]
+  [@@deriving sexp]
+  type coq_BinaryOp = [%import: CrTransformer.coq_BinaryOp]
+  [@@deriving sexp]
+  type coq_HdrOp = [%import: CrTransformer.coq_HdrOp]
+  [@@deriving sexp]
+  type coq_MatchPattern = [%import: CrTransformer.coq_MatchPattern]
+  [@@deriving sexp]
+  type coq_SeqRule = [%import: CrTransformer.coq_SeqRule]
+  [@@deriving sexp]
+  type coq_ParRule = [%import: CrTransformer.coq_ParRule]
+  [@@deriving sexp]
+  type coq_MatchActionRule = [%import: CrTransformer.coq_MatchActionRule]
+  [@@deriving sexp]
+  type coq_Transformer = [%import: CrTransformer.coq_Transformer]
+  [@@deriving sexp]
+end
+include CrDsl
+type coq_CaracaraProgram = [%import: CrDsl.coq_CaracaraProgram]
+[@@deriving sexp]
+
+module CrMem = struct
+  type var_id = [%import : CrMem.var_id]
+  [@@deriving sexp]
+  type coq_Imm = [%import: CrMem.coq_Imm]
+  [@@deriving sexp]
+  type coq_FnArg = [%import: CrMem.coq_FnArg]
+  [@@deriving sexp]
+  type coq_ArithBinOp = [%import: CrMem.coq_ArithBinOp]
+  [@@deriving sexp]
+  type coq_Instruction = [%import: CrMem.coq_Instruction]
+  [@@deriving sexp]
+  type coq_ValType = [%import: CrMem.coq_ValType]
+  [@@deriving sexp]
+  type coq_IM_Program = [%import: CrMem.coq_IM_Program]
+  [@@deriving sexp]
+
+  type arith_expr = [%import: CrMem.arith_expr]
+  and ptr_expr = [%import: CrMem.ptr_expr]
+  and arr_expr = [%import: CrMem.arr_expr]
+  and bool_expr = [%import: CrMem.bool_expr]
+  and coq_Z3Expr = [%import: CrMem.coq_Z3Expr]
+  [@@deriving sexp]
+end
