extracted_code/RunTests.ml
@@ -5,71 +5,169 @@ let get_program f =
   let len = in_channel_length x in
   let str = really_input_string x len in
   close_in x;
-  str |> Sexp.of_string |> Interface.coq_CaracaraProgram_of_sexp
+  str |> Sexp.of_string |> CrTypeIF.coq_CaracaraProgram_of_sexp
 
-let programs = [|
-  get_program "./test/prog1.out";
-  get_program "./test/prog2.out";
-  get_program "./test/subtract1.out"; (* -2*)
-  get_program "./test/subtract2.out";
-  get_program "./test/complex1a.out"; (* -1, +2*)
-  get_program "./test/complex1b.out"; (* +2, -1*)
-|]
+let get_mem_program f =
+  let x = open_in f in
+  let len = in_channel_length x in
+  let str = really_input_string x len in
+  close_in x;
+  str |> Sexp.of_string |> CrTypeIF.CrMem.coq_IM_Program_of_sexp
 
 let tests = ref []
 let register test_label test_fn =
   tests := (test_label, test_fn) :: !tests
 
+(* Test 1:
+ * A program should be equal to itself
+ *)
 let () = register "refl_0" (fun () ->
-  let p = programs.(0) in
+  let p = get_program "./test/prog1.out" in
 
-  let res = SmtQuery.equivalence_checker_cr_dsl p p in
-  match res with
+  match SmtQuery.equivalence_checker_cr_dsl p p with
   | Equivalent -> 1
   | _ -> 0)
 
+(* Test 2:
+ * Different values get statically assigned to header variable
+ * p1: x=5
+ * p2: x=1
+ *)
 let () = register "hdr_diff" (fun () ->
-  let p1 = programs.(0) in
-  let p2 = programs.(1) in
+  let p1 = get_program "./test/prog1.out" in
+  let p2 = get_program "./test/prog2.out" in
 
-  let res = SmtQuery.equivalence_checker_cr_dsl p1 p2 in
-  match res with
+  match SmtQuery.equivalence_checker_cr_dsl p1 p2 with
   | NotEquivalent _ -> 1
   | _ -> 0)
 
-let () = register "refl_1" (fun () ->
-  let p = programs.(2) in
-
-  let res = SmtQuery.equivalence_checker_cr_dsl p p in
-  match res with
-  | Equivalent -> 1
-  | _ -> 0)
-
+(* Test 3:
+ * -1 and +254 should be the same under 8-bit 2s complement
+ * p1: x-1
+ * p2: x+254
+ *)
 let () = register "sub_1comp" (fun () ->
-  let p1 = programs.(2) in
-  let p2 = programs.(3) in
+  let p1 = get_program "./test/subtract1.out" in
+  let p2 = get_program "./test/subtract2.out" in
 
-  let res = SmtQuery.equivalence_checker_cr_dsl p1 p2 in
-   match res with
+  match SmtQuery.equivalence_checker_cr_dsl p1 p2 with
   | Equivalent -> 1
   | _ -> 0)
 
+(* Test 4:
+ * In essence, we're testing that addition is commutative
+ * p1: x - 1 + 2
+ * p2: x + 2 - 1
+ *)
 let () = register "complex_add/sub equal" (fun () ->
-  let p1 = programs.(4) in
-  let p2 = programs.(5) in
+  let p1 = get_program "./test/complex1a.out" in
+  let p2 = get_program "./test/complex1b.out" in
 
-  let res = SmtQuery.equivalence_checker_cr_dsl p1 p2 in
-   match res with
+  match SmtQuery.equivalence_checker_cr_dsl p1 p2 with
   | Equivalent -> 1
   | _ -> 0)
 
+(* Test 5:
+ * Trivially non-equivalent
+ * p1: x + 2 - 1
+ * p2: x - 1
+ *)
 let () = register "complex_add/sub NOT equal" (fun () ->
-  let p1 = programs.(5) in
-  let p2 = programs.(2) in
+  let p1 = get_program "./test/complex1b.out" in
+  let p2 = get_program "./test/subtract1.out" in
 
-  let res = SmtQuery.equivalence_checker_cr_dsl p1 p2 in
-  match res with
+  match SmtQuery.equivalence_checker_cr_dsl p1 p2 with
   | NotEquivalent _ -> 1
+  | _ -> 0)
+
+(* Test 6:
+ * Address offsets should alias
+ * p1: *(x+4)
+ * p2: *(x+2+2)
+ *)
+let () = register "basic address alias" (fun () ->
+  let p1 = get_mem_program "./test/mem1a.out" in
+  let p2 = get_mem_program "./test/mem1b.out" in
+
+  match MemSolver.mem_solve p1 p2 with
+  | Z3Unsat -> 1
+  | _ -> 0)
+
+(* Test 7:
+ * writing a variable value will not always be the same as writing a constant value
+ * p1: *(x+4) = y
+ * p2: *(x+4) = 1
+ *)
+let () = register "basic memory overwrite" (fun () ->
+  let p1 = get_mem_program "./test/mem1a.out" in
+  let p2 = get_mem_program "./test/mem1c.out" in
+
+  match MemSolver.mem_solve p1 p2 with
+  | Z3Sat (_, _, f) -> (
+    match f with
+    | ValueMismatch -> 1
+    | _ -> 0
+    )
+  | _ -> 0)
+
+(* Test 8:
+ * Programs can have different segfault behavior
+ * p1: ret *(x+0)
+ * p2: *(x+1); ret *(x+0)
+ *)
+let () = register "divergent load extents" (fun () ->
+  let p1 = get_mem_program "./test/mem2a.out" in
+  let p2 = get_mem_program "./test/mem2b.out" in
+
+  match MemSolver.mem_solve p1 p2 with
+  | Z3Sat (_, _, f) -> (
+    match f with
+    | BoundsMismatch -> 1
+    | _ -> 0
+    )
+  | _ -> 0)
+
+(* Test 9:
+ * Access extents are the same, and output variables are same
+ * p1: *(x+1); ret *(x+0)
+ * p2: *(x+1)=0; ret *(x+0)
+ *)
+let () = register "mem nop are equiv" (fun () ->
+  let p1 = get_mem_program "./test/mem2b.out" in
+  let p2 = get_mem_program "./test/mem2c.out" in
+
+  match MemSolver.mem_solve p1 p2 with
+  | Z3Unsat -> 1
+  | _ -> 0)
+
+(* Test 10:
+ * If statement collapses
+ * p1: if (0 == 0) then A else B
+ * p2: A
+ *)
+let () = register "degenerate branch" (fun () ->
+  let p1 = get_mem_program "./test/mem3a.out" in
+  let p2 = get_mem_program "./test/mem3b.out" in
+
+  match MemSolver.mem_solve p1 p2 with
+  | Z3Unsat -> 1
+  | _ -> 0)
+
+(* Test 11:
+ * Array values might be different
+ * p1: *(x+1); ret *(x+0)
+ * p2: *(x+0); ret *(x+1)
+ *)
+let () = register "sat aval" (fun () ->
+  let p1 = get_mem_program "./test/mem4a.out" in
+  let p2 = get_mem_program "./test/mem4b.out" in
+  
+  match MemSolver.mem_solve p1 p2 with
+  | Z3Sat (_, _, f) -> (
+    match f with
+    | ValueMismatch -> 1
+    | _ -> 0
+    )
   | _ -> 0)
 
 let () =
