extracted_code/Shim.ml
@@ -1,59 +1,3 @@
-module BinNums = struct
-  include BinNums
-  type positive = [%import: BinNums.positive]
-  [@@deriving sexp]
-  type coq_Z = [%import: BinNums.coq_Z]
-  [@@deriving sexp]
-end
-module Datatypes = struct
-  include Datatypes
-  type ('a, 'b) prod = [%import: ('a, 'b) Datatypes.prod]
-  [@@deriving sexp]
-  type 'a list = [%import: 'a Datatypes.list]
-  [@@deriving sexp]
-end
-module Integers = struct
-  include Integers
-  type bit_int = [%import: Integers.bit_int]
-  [@@deriving sexp]
-end
-module MyInts = struct
-  include MyInts
-  type uint8 = [%import: MyInts.uint8]
-  [@@deriving sexp]
-end
-
-module CrIdentifiers = struct
-  include CrIdentifiers
-  type coq_Header = [%import: CrIdentifiers.coq_Header]
-  [@@deriving sexp]
-  type coq_State = [%import: CrIdentifiers.coq_State]
-  [@@deriving sexp]
-  type coq_Ctrl = [%import: CrIdentifiers.coq_Ctrl]
-  [@@deriving sexp]
-end
-module CrTransformer = struct
-  include CrTransformer
-  type coq_FunctionArgument = [%import: CrTransformer.coq_FunctionArgument]
-  [@@deriving sexp]
-  type coq_BinaryOp = [%import: CrTransformer.coq_BinaryOp]
-  [@@deriving sexp]
-  type coq_HdrOp = [%import: CrTransformer.coq_HdrOp]
-  [@@deriving sexp]
-  type coq_MatchPattern = [%import: CrTransformer.coq_MatchPattern]
-  [@@deriving sexp]
-  type coq_SeqRule = [%import: CrTransformer.coq_SeqRule]
-  [@@deriving sexp]
-  type coq_ParRule = [%import: CrTransformer.coq_ParRule]
-  [@@deriving sexp]
-  type coq_MatchActionRule = [%import: CrTransformer.coq_MatchActionRule]
-  [@@deriving sexp]
-  type coq_Transformer = [%import: CrTransformer.coq_Transformer]
-  [@@deriving sexp]
-end
-include CrDsl
-type coq_CaracaraProgram = [%import: CrDsl.coq_CaracaraProgram]
-[@@deriving sexp]
 
 (* Trusted Shim Procedures *)
 include Integers
@@ -61,16 +5,16 @@ include Datatypes
 include MyInts
 include String
 type coq_ValueMap =
-| VMap of string * uint8 * coq_ValueMap
+| VMap of string * CrVal.coq_CrVal * coq_ValueMap
 | VMap_DNE
-let rec coq_TraverseMap (vm : coq_ValueMap) (s : string) : uint8 =
+let rec coq_TraverseMap (vm : coq_ValueMap) (s : string) : CrVal.coq_CrVal =
   match vm with
   | VMap (var_, val_, nxt_) ->
     if (s = var_) then
       val_
     else
       coq_TraverseMap nxt_ s
-  | VMap_DNE -> repr (Coq_xO (Coq_xO (Coq_xO Coq_xH))) Z0
+  | VMap_DNE -> UninitVal
 let coq_Z_to_int (n : BinNums.coq_Z) : int =
   let rec pos_to_int_ (n : BinNums.positive) (i : int) : int =
     match n with
@@ -82,15 +26,28 @@ let coq_Z_to_int (n : BinNums.coq_Z) : int =
   | Z0 -> 0
   | Zpos n_ -> pos_to_int n_
   | Zneg n_ -> 0 - (pos_to_int n_)
-let int_to_coq_uint8 (n : int) : BinNums.coq_Z =
-  let rec int_to_pos (n : int) : BinNums.positive =
-    if (n = 1) then Coq_xH
-    else if (n mod 2 = 0) then
-      Coq_xO (int_to_pos (n lsr 1))
-    else
-      Coq_xI (int_to_pos (n lsr 1)) in
+let rec pos_to_str (n : BinNums.positive) : Stdlib.String.t =
+  match n with
+  | Coq_xH -> "1"
+  | Coq_xO n_ -> (pos_to_str n_) ^ "0"
+  | Coq_xI n_ -> (pos_to_str n_) ^ "1"
 
+let rec int_to_pos (n : int) : BinNums.positive =
+  if (n = 1) then Coq_xH
+  else if (n mod 2 = 0) then
+    Coq_xO (int_to_pos (n lsr 1))
+  else
+    Coq_xI (int_to_pos (n lsr 1))
+let int_to_coq_uint8 (n : int) : BinNums.coq_Z =
   repr (Coq_xO (Coq_xO (Coq_xO Coq_xH))) (
+    if (n = 0) then Z0
+    else Zpos (int_to_pos n))
+let int_to_coq_uint32 (n : int) : BinNums.coq_Z =
+  repr (Coq_xO (Coq_xO (Coq_xO (Coq_xO (Coq_xO Coq_xH))))) (
+    if (n = 0) then Z0
+    else Zpos (int_to_pos n))
+let int_to_coq_uint64 (n : int) : BinNums.coq_Z =
+  repr (Coq_xO (Coq_xO (Coq_xO (Coq_xO (Coq_xO (Coq_xO Coq_xH)))))) (
     if (n = 0) then Z0
     else Zpos (int_to_pos n))
 let rec coq_str_to_str (s : string) : Stdlib.String.t =
