extracted_code/Z3Solver.ml
@@ -21,9 +21,15 @@ let rec z3_expr_from_coq_smt_bool_expr (expr : SmtExpr.coq_SmtBoolExpr) (ctx : Z
 and z3_expr_from_coq_smt_arith_expr (expr : SmtExpr.coq_SmtArithExpr) (ctx : Z3.context) (vars : var_tracker)
   : Z3.Expr.expr =
   match expr with
-  | SmtExpr.SmtConst n -> Z3.BitVector.mk_numeral ctx (string_of_int (Interface.coq_Z_to_int n)) 8
+  | SmtExpr.SmtArithConst n -> (
+      match n with
+      | CrVal.CrUInt8 val8 -> Z3.BitVector.mk_numeral ctx (string_of_int (Shim.coq_Z_to_int val8)) 8
+      | CrVal.CrUInt16 val16 -> Z3.BitVector.mk_numeral ctx (string_of_int (Shim.coq_Z_to_int val16)) 16
+      | CrVal.CrUInt32 val32 -> Z3.BitVector.mk_numeral ctx (string_of_int (Shim.coq_Z_to_int val32)) 32
+      | CrVal.CrUInt64 val64 -> Z3.BitVector.mk_numeral ctx (string_of_int (Shim.coq_Z_to_int val64)) 64
+      | CrVal.CrNilInt -> Z3.BitVector.mk_numeral ctx "0" 8)
   | SmtExpr.SmtArithVar name -> (
-    let name_str = Interface.coq_str_to_str name in
+    let name_str = Shim.coq_str_to_str name in
     match StringMap.find_opt name_str !vars with
     | Some z3_var -> z3_var
     | None ->
@@ -41,21 +47,48 @@ and z3_expr_from_coq_smt_arith_expr (expr : SmtExpr.coq_SmtArithExpr) (ctx : Z3.
   | SmtExpr.SmtBitMul (e1, e2) -> Z3.BitVector.mk_mul ctx (z3_expr_from_coq_smt_arith_expr e1 ctx vars) (z3_expr_from_coq_smt_arith_expr e2 ctx vars)
   | SmtExpr.SmtBitDiv (e1, e2) -> Z3.BitVector.mk_udiv ctx (z3_expr_from_coq_smt_arith_expr e1 ctx vars) (z3_expr_from_coq_smt_arith_expr e2 ctx vars)
   | SmtExpr.SmtBitMod (e1, e2) -> Z3.BitVector.mk_smod ctx (z3_expr_from_coq_smt_arith_expr e1 ctx vars) (z3_expr_from_coq_smt_arith_expr e2 ctx vars)
+  | SmtExpr.SmtArrSel (_, _, _) -> 
+      (* TODO: Implement pointer load from memory *)
+      Z3.BitVector.mk_numeral ctx "0" 8
+  | SmtExpr.SmtPtrConst ptr -> (
+      match ptr with
+      | CrVal.CrPtr addr -> Z3.BitVector.mk_numeral ctx (string_of_int (Shim.coq_Z_to_int addr)) 64
+      | CrVal.CrNilPtr -> Z3.BitVector.mk_numeral ctx "0" 64)
+  | SmtExpr.SmtPtrVar name -> (
+      let name_str = Shim.coq_str_to_str name in
+      match StringMap.find_opt name_str !vars with
+      | Some z3_var -> z3_var
+      | None ->
+          let z3_var = Z3.BitVector.mk_const ctx (Z3.Symbol.mk_string ctx name_str) 64 in
+          vars := StringMap.add name_str z3_var !vars;
+          z3_var)
 
 (* Gets all variable assignments and folds them into a valuation (linked list) *)
-let to_vmap (m : Z3.Model.model) (acc : Interface.coq_ValueMap) (name : string) (z3_var : Z3.Expr.expr) : Interface.coq_ValueMap =
+let to_vmap (m : Z3.Model.model) (acc : Shim.coq_ValueMap) (name : string) (z3_var : Z3.Expr.expr) : Shim.coq_ValueMap =
   match Z3.Model.eval m z3_var true with
   | Some v ->
     if Z3.Expr.is_numeral v then
+      let bv_size = Z3.BitVector.get_size (Z3.Expr.get_sort v) in
       let var_str = Z3.BitVector.numeral_to_string v in
       let var_val = int_of_string var_str in
       Printf.printf "| var( \027[1m%s\027[0m ) := %d\n" name var_val;
-      Interface.VMap (
-        Interface.str_to_coq_str name,
-        Interface.int_to_coq_uint8 var_val,
+      (* TODO: Better casting *)
+      let cr_val = 
+        if bv_size = 8 then
+          CrVal.IntVal (CrVal.CrUInt8 (Shim.int_to_coq_uint8 var_val))
+        else if bv_size = 32 then
+          CrVal.IntVal (CrVal.CrUInt32 (Shim.int_to_coq_uint32 var_val))
+        else if bv_size = 64 then
+          CrVal.PtrVal (CrVal.CrPtr (Shim.int_to_coq_uint64 var_val))
+        else
+          CrVal.UninitVal
+      in
+      Shim.VMap (
+        Shim.str_to_coq_str name,
+        cr_val,
         acc)
     else
-      raise (Failure ("Expects uint8 but got non-numeral value for " ^ name))
+      raise (Failure ("Expects uint but got non-numeral value for " ^ name))
   | None -> raise (Failure ("Z3 failed to return valuation for " ^ name))
 
 let sat_check solver tracked_vars =
@@ -70,10 +103,10 @@ let sat_check solver tracked_vars =
       let var_bindings = StringMap.bindings !tracked_vars in
       let valuations = Stdlib.List.fold_left
         (fun acc (name, z3_var) -> to_vmap m acc name z3_var)
-        Interface.VMap_DNE
+        Shim.VMap_DNE
         var_bindings in
       Printf.printf "└\n";
-      SmtTypes.SmtSat (Interface.coq_TraverseMap valuations))
+      SmtTypes.SmtSat (Shim.coq_TraverseMap valuations))
     | None -> raise (Failure "Z3 returned SAT, but no valuation."))
 
 let solve (expr : SmtExpr.coq_SmtBoolExpr) =
@@ -83,4 +116,4 @@ let solve (expr : SmtExpr.coq_SmtBoolExpr) =
   let z3_expr = z3_expr_from_coq_smt_bool_expr expr ctx tracked_vars in
   Solver.add solver [z3_expr];
 
-  sat_check solver tracked_vars
+  sat_check solver tracked_vars 
