SmtTypes.v
@@ -1,12 +1,12 @@
 From Coq.Strings Require Import String.
-From MyProject Require Import MyInts.
+From MyProject Require Import CrVal.
 
 (* Note that these strings may or may not have a one-to-one correspondence with
   identifiers in the CrDsl program. *)
 (* Currently only need valuations from strings to uint8
   because there are no primitive bool variables within the IR.
   Expressions can still be bools though (for conditionals, equalities, etc.) *)
-Definition SmtValuation := string -> uint8.
+Definition SmtValuation := string -> CrVal.
 
 Inductive SmtResult : Type :=
   | SmtSat (f : SmtValuation)  (* Satisfiable with valuation f *)
