CrMem.v
@@ -1,0 +1,821 @@
+(* TODO: Add Comments *)
+
+Require Import ZArith.
+From Coq.Strings Require Import String.
+From Coq.Strings Require Import Ascii.
+Require Import List.
+Import ListNotations.
+From MyProject Require Import CrVal.
+From MyProject Require Import CrIdentifiers.
+From MyProject Require Import SmtExpr.
+From MyProject Require Import Maps.
+From MyProject Require Import Integers.
+From MyProject Require Import MyInts.
+
+Inductive ValType : Type :=
+| uint8_t
+| uint32_t
+| uintptr_t
+| array_t
+| nil_t
+| err_t.
+
+Definition var_id := positive.
+Inductive Imm : Type :=
+| imm_u8 (v : uint8)
+| imm_u32 (v : uint32)
+| imm_ptr (b : uintbptr).
+Inductive FnArg : Type :=
+| IOArg (vid : var_id)
+| TmpArg (tid : var_id)
+| ValArg (v : Imm).
+Inductive ArithBinOp : Type :=
+| AddOp
+| SubOp
+| ASLOp
+| ASROp
+| BitAndOp
+| BitOrOp
+| BitXorOp.
+Inductive Instruction : Type :=
+| AllocOp (dst a1 a2 : FnArg)
+| LdOp (dst a1 a2 : FnArg)
+| StOp (a1 a2 a3 : FnArg)
+| Binary (op : ArithBinOp) (dst a1 a2 : FnArg)
+| BitFlipOp (dst a1 : FnArg)
+| BrzOp (cond : FnArg) (zero_br : list Instruction) (nonzero_br : list Instruction).
+Record IM_Program := {
+  fn_in : list (var_id * ValType);
+  fn_body : list Instruction;
+  fn_out_vars : list var_id;
+  fn_out_iaddrs : list (uintbptr * uint32);
+  fn_out_vaddrs : list (var_id * uint32);
+}.
+
+Definition HasError : Type := bool.
+Definition TypedExpr (T : Type) : Type := ValType * T.
+Record machine_state {T : Type} := {
+  io_map : PMap.t (TypedExpr T);
+  tmp_map : PMap.t (TypedExpr T);
+  iarr_map : PMap.t (TypedExpr T);
+  varr_map : PMap.t (TypedExpr T);
+  bound_map : PMap.t (TypedExpr T);
+  flag : HasError;
+}.
+Arguments machine_state T : clear implicits.
+Definition set_io {T : Type} (m : machine_state T) (k : positive) (v : ValType * T) := {|
+  io_map := PMap.set k v (io_map m);
+  tmp_map := tmp_map m; iarr_map := iarr_map m; varr_map := varr_map m; bound_map := bound_map m; flag := flag m;
+|}.
+Definition set_tmp {T : Type} (m : machine_state T) (k : positive) (v : ValType * T) := {|
+  tmp_map := PMap.set k v (tmp_map m);
+  io_map := io_map m; iarr_map := iarr_map m; varr_map := varr_map m; bound_map := bound_map m; flag := flag m;
+|}.
+Definition set_iarr {T : Type} (m : machine_state T) (k : positive) (v : ValType * T) := {|
+  iarr_map := PMap.set k v (iarr_map m);
+  io_map := io_map m; tmp_map := tmp_map m; varr_map := varr_map m; bound_map := bound_map m; flag := flag m;
+|}.
+Definition set_varr {T : Type} (m : machine_state T) (k : positive) (v : ValType * T) := {|
+  varr_map := PMap.set k v (varr_map m);
+  io_map := io_map m; tmp_map := tmp_map m; iarr_map := iarr_map m; bound_map := bound_map m; flag := flag m;
+|}.
+Definition set_bound {T : Type} (m : machine_state T) (k : positive) (v : ValType * T) := {|
+  bound_map := PMap.set k v (bound_map m);
+  io_map := io_map m; tmp_map := tmp_map m; iarr_map := iarr_map m; varr_map := varr_map m; flag := flag m;
+|}.
+Definition set_flag {T : Type} (m : machine_state T) (b : bool) := {|
+  flag := b;
+  io_map := io_map m; tmp_map := tmp_map m; iarr_map := iarr_map m; varr_map := varr_map m; bound_map := bound_map m;
+|}.
+
+Inductive arith_expr :=
+| Z3_int8 (x : uint8)
+| Z3_int32 (x : uint32)
+| Z3_int8_var (name : positive)
+| Z3_int32_var (name : positive)
+| Z3_bv_add (e1 e2 : arith_expr)
+| Z3_bv_sub (e1 e2 : arith_expr)
+| Z3_bv_shl (e1 e2 : arith_expr)
+| Z3_bv_ashr (e1 e2 : arith_expr)
+| Z3_bv_and (e1 e2 : arith_expr)
+| Z3_bv_or (e1 e2 : arith_expr)
+| Z3_bv_xor (e1 e2 : arith_expr)
+| Z3_bv_not (e : arith_expr)
+| Z3_arr_sel (e1 : arr_expr) (e2 : arith_expr)
+| Z3_arith_ite (c : bool_expr) (e1 e2 : arith_expr)
+with ptr_expr :=
+| Z3_ptr (x : uintbptr)
+| Z3_ptr_var (name : positive)
+| Z3_ptr_ite (c : bool_expr) (e1 e2 : ptr_expr)
+with arr_expr :=
+| Z3_arr_init (len : arith_expr)
+| Z3_arr_var (name : positive)
+| Z3_arr_st (A : arr_expr) (idx : arith_expr) (item : arith_expr)
+| Z3_arr_ite (c : bool_expr) (e1 e2 : arr_expr)
+with bool_expr :=
+| Z3_T
+| Z3_F
+| Z3_Neg (e : bool_expr)
+| Z3_Conj (e1 e2 : bool_expr)
+| Z3_Disj (e1 e2 : bool_expr)
+| Z3_Eq (e1 e2 : Z3Expr)
+| Z3_Lt (e1 e2 : arith_expr)
+with Z3Expr :=
+| Z3Arith (e : arith_expr)
+| Z3Ptr (e : ptr_expr)
+| Z3Array (e : arr_expr)
+| Z3Bool (e : bool_expr)
+| Z3Nil.
+
+Definition sym_state := machine_state Z3Expr.
+Definition init_sym : sym_state := {|
+  io_map := PMap.init (nil_t, Z3Nil);
+  tmp_map := PMap.init (nil_t, Z3Nil);
+  iarr_map := PMap.init (nil_t, Z3Nil);
+  varr_map := PMap.init (nil_t, Z3Nil);
+  bound_map := PMap.init (nil_t, Z3Nil);
+  flag := false;
+|}.
+
+Fixpoint apply_io_helper (io : PMap.t (TypedExpr Z3Expr)) (input : list (positive * ValType)) : PMap.t (TypedExpr Z3Expr) :=
+  match input with
+  | [] => io
+  | (k, uint8_t) :: rest =>
+    apply_io_helper (PMap.set k (uint8_t, Z3Arith (Z3_int8_var k)) io) rest
+  | (k, uint32_t) :: rest =>
+    apply_io_helper (PMap.set k (uint32_t, Z3Arith (Z3_int32_var k)) io) rest
+  | (k, uintptr_t) :: rest =>
+    apply_io_helper (PMap.set k (uintptr_t, Z3Ptr (Z3_ptr_var k)) io) rest
+  | (k, _) :: rest => apply_io_helper (PMap.set k (err_t, Z3Nil) io) rest
+  end.
+Fixpoint apply_varr_helper (varr : PMap.t (TypedExpr Z3Expr)) (input : list (positive * ValType)) : PMap.t (TypedExpr Z3Expr) :=
+  match input with
+  | [] => varr
+  | (k, uintptr_t) :: rest =>
+    apply_varr_helper (PMap.set k (array_t, Z3Array (Z3_arr_var k)) varr) rest
+  | _ :: rest => apply_varr_helper varr rest
+  end.
+Definition apply_input (m : sym_state) (iv : list (positive * ValType)) : sym_state := {|
+  io_map := apply_io_helper (io_map init_sym) iv;
+  tmp_map := tmp_map init_sym;
+  iarr_map := iarr_map init_sym;
+  varr_map := apply_varr_helper (varr_map init_sym) iv;
+  bound_map := bound_map init_sym;
+  flag := flag init_sym;
+|}.
+
+Definition sym_interp_arg (m : sym_state) (a : FnArg) : TypedExpr Z3Expr :=
+  match a with
+  | IOArg x => (io_map m) !! x
+  | TmpArg x => (tmp_map m) !! x
+  | ValArg x =>
+    match x with
+    | imm_u8 x' => (uint8_t, Z3Arith (Z3_int8 x'))
+    | imm_u32 x' => (uint32_t, Z3Arith (Z3_int32 x'))
+    | imm_ptr x' => (uintptr_t, Z3Ptr (Z3_ptr x'))
+    end
+  end.
+
+Definition uptr_to_key (p : uintbptr) : positive :=
+  Pos.of_nat (S (Z.to_nat (unsigned p))).
+
+Definition sym_alloc (m : sym_state) (dst a1 a2: FnArg) :=
+  let local_lookup := sym_interp_arg m in
+  let m' :=
+    match local_lookup a2 with
+    | (uint32_t, Z3Arith e2) =>
+      match local_lookup a1 with
+      | (uintptr_t, Z3Ptr (Z3_ptr x)) =>
+        (set_iarr m (uptr_to_key x) (array_t, Z3Array (Z3_arr_init e2)))
+      | (uintptr_t, Z3Ptr (Z3_ptr_var x)) =>
+        (set_varr m x (array_t, Z3Array (Z3_arr_init e2)))
+      | _ => set_flag m true
+      end
+    | _ => set_flag m true
+    end
+  in
+  match dst with
+  | IOArg x => set_io m' x (local_lookup a1)
+  | TmpArg x => set_tmp m' x (local_lookup a1)
+  | _ => set_flag m' true
+  end.
+
+Definition get_sym_ld_val (m : sym_state) (dst : FnArg) (e1 : ptr_expr) (e2 : arith_expr) :=
+  let lookup := match e1 with
+  | Z3_ptr x =>
+    (iarr_map m) !! (uptr_to_key x)
+  | Z3_ptr_var x =>
+    (varr_map m) !! x
+  | Z3_ptr_ite _ _ _ => (err_t, Z3Nil)
+  end in
+  let val := match lookup with
+  | (array_t, Z3Array A) => (uint8_t, Z3Arith (Z3_arr_sel A e2))
+  | _ => (err_t, Z3Nil)
+  end in
+  let m' := match e1 with 
+  | Z3_ptr_var x => match (bound_map m) !! x with
+    | (uint32_t, Z3Arith prev_bound) =>
+        set_bound m x
+        (uint32_t, Z3Arith (Z3_arith_ite
+          (Z3_Lt e2 prev_bound)
+          prev_bound
+          e2))
+    | _ => set_bound m x (uint32_t, Z3Arith e2)
+    end
+  | _ => m
+  end in
+  match val, dst with
+  | (uint8_t, Z3Arith _), IOArg x => set_io m' x val
+  | (uint8_t, Z3Arith _), TmpArg x => set_tmp m' x val
+  | _, _ => set_flag m true
+  end.
+Definition sym_ld (m : sym_state) (dst a1 a2 : FnArg) :=
+  let local_lookup := sym_interp_arg m in
+  let '(a1_t, a1_v) := local_lookup a1 in
+  let '(a2_t, a2_v) := local_lookup a2 in
+  match a1_t, a1_v, a2_t, a2_v with
+  | uintptr_t, Z3Ptr e1, uint32_t, Z3Arith e2 =>
+    get_sym_ld_val m dst e1 e2
+  | _, _, _, _ => set_flag m true
+  end.
+
+Definition sym_st (m : sym_state) (a1 a2 a3 : FnArg) :=
+  let local_lookup := sym_interp_arg m in
+  (* TODO: handle case where a1 is a ValArg imm_ptr *)
+  let st_idx := match local_lookup a2 with
+  | (uint32_t, Z3Arith e2) => (uint32_t, Z3Arith e2)
+  | _ => (err_t, Z3Nil)
+  end in
+  let st_val := match local_lookup a3 with
+  | (uint8_t, Z3Arith e3) => (uint8_t, Z3Arith e3)
+  | _ => (err_t, Z3Nil)
+  end in
+  match local_lookup a1, st_idx, st_val with
+  | (uintptr_t, Z3Ptr (Z3_ptr x)), (uint32_t, Z3Arith e2), (uint8_t, Z3Arith e3) =>
+    match (iarr_map m) !! (uptr_to_key x) with
+    | (array_t, Z3Array A) =>
+      set_iarr m (uptr_to_key x) (array_t, Z3Array (Z3_arr_st A e2 e3))
+    | _ => set_flag m true
+    end
+  | (uintptr_t, Z3Ptr (Z3_ptr_var x)), (uint32_t, Z3Arith e2), (uint8_t, Z3Arith e3) =>
+    match (varr_map m) !! x with
+    | (array_t, Z3Array A) =>
+      match (bound_map m) !! x with
+      | (uint32_t, Z3Arith prev_bound) =>
+          set_varr (set_bound m x
+            (uint32_t, Z3Arith (Z3_arith_ite
+              (Z3_Lt e2 prev_bound)
+              prev_bound
+              e2))) x (array_t, Z3Array (Z3_arr_st A e2 e3))
+      | _ => set_varr (set_bound m x st_idx) x (array_t, Z3Array (Z3_arr_st A e2 e3))
+      end
+    | _ => set_flag m true
+    end
+  | _, _, _ => set_flag m true
+  end.
+
+Definition set_ (dst : FnArg) (m : sym_state) (val : TypedExpr Z3Expr) :=
+  match val, dst with
+  | (err_t, _), _ => set_flag m true
+  | _, IOArg x => set_io m x val
+  | _, TmpArg x => set_tmp m x val
+  | _, ValArg _ => set_flag m true
+  end.
+
+Definition bin_to_expr (op : ArithBinOp) (e1 e2 : arith_expr) : Z3Expr :=
+  match op with
+  | AddOp => Z3Arith (Z3_bv_add e1 e2)
+  | SubOp => Z3Arith (Z3_bv_sub e1 e2)
+  | ASLOp => Z3Arith (Z3_bv_shl e1 e2)
+  | ASROp => Z3Arith (Z3_bv_ashr e1 e2)
+  | BitAndOp => Z3Arith (Z3_bv_and e1 e2)
+  | BitOrOp => Z3Arith (Z3_bv_or e1 e2)
+  | BitXorOp => Z3Arith (Z3_bv_xor e1 e2)
+  end.
+
+Definition sym_binop (m : sym_state) (op : ArithBinOp) (dst a1 a2 : FnArg) :=
+  let local_lookup := sym_interp_arg m in
+  let new_val : TypedExpr Z3Expr :=
+  match local_lookup a1, local_lookup a2 with
+  | (uint8_t, Z3Arith e1), (uint8_t, Z3Arith e2) =>
+    (uint8_t, bin_to_expr op e1 e2)
+  | (uint32_t, Z3Arith e1), (uint32_t, Z3Arith e2) =>
+    (uint32_t, bin_to_expr op e1 e2)
+  | (_, e1), _ => (err_t, e1)
+  end in
+  set_ dst m new_val.
+
+Definition sym_bitflip (m : sym_state) (dst a1 : FnArg) :=
+  let local_lookup := sym_interp_arg m in
+  let new_val : TypedExpr Z3Expr :=
+  match local_lookup a1 with
+  | (uint8_t, Z3Arith e1) =>
+    (uint8_t, Z3Arith (Z3_bv_not e1))
+  | (uint32_t, Z3Arith e1) =>
+    (uint32_t, Z3Arith (Z3_bv_not e1))
+  | (_, e1) => (err_t, e1)
+  end in
+  set_ dst m new_val.
+
+Definition get_ite_expr (c : bool_expr) (te1 te2 : TypedExpr Z3Expr) : TypedExpr Z3Expr :=
+  let '(t1, v1) := te1 in
+  let '(t2, v2) := te2 in
+  let ite_expr :=
+  match v1, v2 with
+  | Z3Arith e1, Z3Arith e2 => Z3Arith (Z3_arith_ite c e1 e2)
+  | Z3Ptr e1, Z3Ptr e2 => Z3Ptr (Z3_ptr_ite c e1 e2)
+  | Z3Array e1, Z3Array e2 => Z3Array (Z3_arr_ite c e1 e2)
+  | _, _ => Z3Nil
+  end in
+  match t1, t2 with
+  | err_t, _ => te1
+  | _, err_t => te2
+  | _, _ => (t1, ite_expr)
+  end.
+
+Fixpoint merge_var_maps (c : bool_expr) (keys : list positive)
+    (m1 m2 : PMap.t (TypedExpr Z3Expr)) (acc : PMap.t (TypedExpr Z3Expr)) : PMap.t (TypedExpr Z3Expr) :=
+  match keys with
+  | [] => acc
+  | k :: rest =>
+    let v := get_ite_expr c (m1 !! k) (m2 !! k) in
+    merge_var_maps c rest m1 m2 (PMap.set k v acc)
+  end.
+Definition as_ite (c : bool_expr) (keys : list positive) (m1 m2 : sym_state) : sym_state := {|
+  io_map := merge_var_maps c keys (io_map m1) (io_map m2) (io_map m2);
+  tmp_map := merge_var_maps c keys (tmp_map m1) (tmp_map m2) (tmp_map m2);
+  iarr_map := merge_var_maps c keys (iarr_map m1) (iarr_map m2) (iarr_map m2);
+  varr_map := merge_var_maps c keys (varr_map m1) (varr_map m2) (varr_map m2);
+  bound_map := merge_var_maps c keys (bound_map m1) (bound_map m2) (bound_map m2);
+  flag := orb (flag m1) (flag m2);
+|}.
+
+Fixpoint collect_dst_keys_instr (i : Instruction) : list positive :=
+  let dst_key_of := fun a => match a with IOArg x | TmpArg x => [x] | _ => [] end in
+  let ptr_key_of := fun a => match a with IOArg x | TmpArg x => [x] | _ => [] end in
+  match i with
+  | AllocOp dst a1 _ => dst_key_of dst ++ ptr_key_of a1
+  | LdOp dst a1 _ => dst_key_of dst ++ ptr_key_of a1
+  | StOp a1 _ _ => ptr_key_of a1
+  | Binary _ dst _ _ => dst_key_of dst
+  | BitFlipOp dst _ => dst_key_of dst
+  | BrzOp _ if_z if_nz =>
+    (fix go (l : list Instruction) :=
+      match l with [] => [] | x :: xs => collect_dst_keys_instr x ++ go xs end) if_z
+    ++
+    (fix go (l : list Instruction) :=
+      match l with [] => [] | x :: xs => collect_dst_keys_instr x ++ go xs end) if_nz
+  end.
+Definition collect_dst_keys (instrs : list Instruction) : list positive :=
+  flat_map collect_dst_keys_instr instrs.
+
+Fixpoint apply_sym_op (i : Instruction) (m : sym_state) {struct i} : sym_state :=
+  if (flag m) then
+    m
+  else
+    match i with
+    | AllocOp dst a1 a2 => sym_alloc m dst a1 a2
+    | LdOp dst a1 a2 => sym_ld m dst a1 a2
+    | StOp a1 a2 a3 => sym_st m a1 a2 a3
+    | Binary op dst a1 a2 => sym_binop m op dst a1 a2
+    | BitFlipOp dst a1 => sym_bitflip m dst a1
+    | BrzOp cond zero_br nonzero_br =>
+      let eval_list :=
+        fix go (p : list Instruction) (m : sym_state) : sym_state :=
+          match p with
+          | [] => m
+          | i :: rest => go rest (apply_sym_op i m)
+          end
+      in
+      let local_lookup := sym_interp_arg m in
+      match local_lookup cond with
+      | (uint8_t, Z3Arith cond_e) =>
+        let if_zero := Z3_Eq (Z3Arith cond_e) (Z3Arith (Z3_int8 (repr 0))) in
+        let m_zero := eval_list zero_br m in
+        let m_nonzero := eval_list nonzero_br m in
+        let keys := collect_dst_keys zero_br ++ collect_dst_keys nonzero_br in
+        as_ite if_zero keys m_zero m_nonzero
+      | (uint32_t, Z3Arith cond_e) =>
+        let if_zero := Z3_Eq (Z3Arith cond_e) (Z3Arith (Z3_int32 (repr 0))) in
+        let m_zero := eval_list zero_br m in
+        let m_nonzero := eval_list nonzero_br m in
+        let keys := collect_dst_keys zero_br ++ collect_dst_keys nonzero_br in
+        as_ite if_zero keys m_zero m_nonzero
+      | _ => set_flag m true
+      end
+    end.
+
+Definition sym_eval_helper (p : list Instruction) (m : sym_state) : sym_state :=
+  List.fold_left (fun m' i => apply_sym_op i m') p m.
+
+Record output_valuation {T : Type} : Type := {
+  errored : HasError;
+  var_val : var_id -> TypedExpr T;
+  iptr_val : (uintbptr * uint32) -> TypedExpr T;
+  vptr_val : (var_id * uint32) -> TypedExpr T;
+  vptr_bound : var_id -> TypedExpr T;
+}.
+Arguments output_valuation T : clear implicits.
+
+Definition sym_eval_program (p : IM_Program) : output_valuation Z3Expr :=
+  let m' := sym_eval_helper (fn_body p) (apply_input init_sym (fn_in p)) in {|
+    errored := flag m';
+    var_val := fun k => match (io_map m') !! k with
+      | (nil_t, _) => (nil_t, Z3Nil)
+      | (err_t, _) => (err_t, Z3Nil)
+      | (t, e) => (t, e)
+      end;
+    iptr_val := fun '(b, i) => match (iarr_map m') !! (uptr_to_key b) with
+      | (array_t, Z3Array e) => (uint8_t, Z3Arith (Z3_arr_sel e (Z3_int32 i)))
+      | _ => (err_t, Z3Nil)
+      end;
+    vptr_val := fun '(k, i) => match (varr_map m') !! k with
+      | (array_t, Z3Array e) => (uint8_t, Z3Arith (Z3_arr_sel e (Z3_int32 i)))
+      | _ => (err_t, Z3Nil)
+      end;
+    vptr_bound := fun k => match (bound_map m') !! k with
+      | (uint32_t, Z3Arith e) => (uint32_t, Z3Arith e)
+      | _ => (err_t, Z3Nil)
+      end;
+  |}.
+
+Definition z3_s_val : Type := var_id -> CrVal.
+Definition z3_a_val : Type := var_id -> @Array CrVal.
+
+Definition eval_z3_arith_binop (op : ArithBinOp) (v1 v2 : CrVal) : CrVal :=
+  match v1, v2 with
+  | IntVal (CrUInt8 x1), IntVal (CrUInt8 x2) =>
+    match op with
+    | AddOp => IntVal (CrUInt8 (Integers.add x1 x2))
+    | SubOp => IntVal (CrUInt8 (Integers.sub x1 x2))
+    | ASLOp => IntVal (CrUInt8 (Integers.shl x1 x2))
+    | ASROp => IntVal (CrUInt8 (Integers.shr x1 x2))
+    | BitAndOp => IntVal (CrUInt8 (Integers.and x1 x2))
+    | BitOrOp => IntVal (CrUInt8 (Integers.or x1 x2))
+    | BitXorOp => IntVal (CrUInt8 (Integers.xor x1 x2))
+    end
+  | IntVal (CrUInt32 x1), IntVal (CrUInt32 x2) =>
+    match op with
+    | AddOp => IntVal (CrUInt32 (Integers.add x1 x2))
+    | SubOp => IntVal (CrUInt32 (Integers.sub x1 x2))
+    | ASLOp => IntVal (CrUInt32 (Integers.shl x1 x2))
+    | ASROp => IntVal (CrUInt32 (Integers.shr x1 x2))
+    | BitAndOp => IntVal (CrUInt32 (Integers.and x1 x2))
+    | BitOrOp => IntVal (CrUInt32 (Integers.or x1 x2))
+    | BitXorOp => IntVal (CrUInt32 (Integers.xor x1 x2))
+    end
+  | _, _ => ErrorVal
+  end.
+
+Fixpoint eval_z3_arith (e : arith_expr) (sval : z3_s_val) (aval : z3_a_val) : CrVal :=
+  match e with
+  | Z3_int8 x => IntVal (CrUInt8 x)
+  | Z3_int32 x => IntVal (CrUInt32 x)
+  | Z3_int8_var name
+  | Z3_int32_var name => sval name
+  | Z3_bv_add e1 e2 =>
+    eval_z3_arith_binop AddOp
+      (eval_z3_arith e1 sval aval)
+      (eval_z3_arith e2 sval aval)
+  | Z3_bv_sub e1 e2 =>
+    eval_z3_arith_binop SubOp
+      (eval_z3_arith e1 sval aval)
+      (eval_z3_arith e2 sval aval)
+  | Z3_bv_shl e1 e2 =>
+    eval_z3_arith_binop ASLOp
+      (eval_z3_arith e1 sval aval)
+      (eval_z3_arith e2 sval aval)
+  | Z3_bv_ashr e1 e2 =>
+    eval_z3_arith_binop ASROp
+      (eval_z3_arith e1 sval aval)
+      (eval_z3_arith e2 sval aval)
+  | Z3_bv_and e1 e2 =>
+    eval_z3_arith_binop BitAndOp
+      (eval_z3_arith e1 sval aval)
+      (eval_z3_arith e2 sval aval)
+  | Z3_bv_or e1 e2 =>
+    eval_z3_arith_binop BitOrOp
+      (eval_z3_arith e1 sval aval)
+      (eval_z3_arith e2 sval aval)
+  | Z3_bv_xor e1 e2 =>
+    eval_z3_arith_binop BitXorOp
+      (eval_z3_arith e1 sval aval)
+      (eval_z3_arith e2 sval aval)
+  | Z3_bv_not e1 =>
+    let v := eval_z3_arith e1 sval aval in
+    match v with
+    | IntVal (CrUInt8 x) => IntVal (CrUInt8 (Integers.not x))
+    | IntVal (CrUInt32 x) => IntVal (CrUInt32 (Integers.not x))
+    | _ => ErrorVal
+    end
+  | Z3_arr_sel e1 e2 =>
+    let res := CrVal.ld_arr (eval_z3_array e1 sval aval) (eval_z3_arith e2 sval aval) in
+    match res with
+    | Legal v => v
+    | Illegal => ErrorVal
+    end
+  | Z3_arith_ite c e1 e2 =>
+    match eval_z3_bool c sval aval with
+    | true => eval_z3_arith e1 sval aval
+    | false => eval_z3_arith e2 sval aval
+    end
+  end
+with eval_z3_ptr (e : ptr_expr) (sval : z3_s_val) (aval : z3_a_val) : CrVal :=
+  match e with
+  | Z3_ptr x => PtrVal (CrPtr x)
+  | Z3_ptr_var name => sval name
+  | Z3_ptr_ite c e1 e2 =>
+    match eval_z3_bool c sval aval with
+    | true => eval_z3_ptr e1 sval aval
+    | false => eval_z3_ptr e2 sval aval
+    end
+  end
+with eval_z3_array (e : arr_expr) (sval : z3_s_val) (aval : z3_a_val) : Array :=
+  match e with
+  | Z3_arr_init e1 =>
+    match eval_z3_arith e1 sval aval with
+    | IntVal (CrUInt32 len) =>
+      Allocated {|
+        arr_len := len;
+        arr_bytes := PMap.init Uninit
+      |}
+    | _ => Unallocated
+    end
+  | Z3_arr_var name => aval name
+  | Z3_arr_st A idx item =>
+    let arr := eval_z3_array A sval aval in
+    let i := eval_z3_arith idx sval aval in
+    let v := eval_z3_arith item sval aval in
+    match CrVal.st_arr arr i v with
+    | Legal a' => a'
+    | Illegal => Unallocated
+    end
+  | Z3_arr_ite c e1 e2 =>
+    match eval_z3_bool c sval aval with
+    | true => eval_z3_array e1 sval aval
+    | false => eval_z3_array e2 sval aval
+    end
+  end
+with eval_z3_bool (e : bool_expr) (sval : z3_s_val) (aval : z3_a_val) : bool :=
+  match e with
+  | Z3_T => true
+  | Z3_F => false
+  | Z3_Neg e' => negb (eval_z3_bool e' sval aval)
+  | Z3_Conj e1 e2 => andb (eval_z3_bool e1 sval aval) (eval_z3_bool e2 sval aval)
+  | Z3_Disj e1 e2 => orb (eval_z3_bool e1 sval aval) (eval_z3_bool e2 sval aval)
+  | Z3_Eq e1 e2 =>
+    let v1 := eval_z3_expr e1 sval aval in
+    let v2 := eval_z3_expr e2 sval aval in
+    CrVal.eqb v1 v2
+  | Z3_Lt e1 e2 =>
+    let v1 := eval_z3_arith e1 sval aval in
+    let v2 := eval_z3_arith e2 sval aval in
+    CrVal.ltb v1 v2
+  end
+with eval_z3_expr (e : Z3Expr) (sval : z3_s_val) (aval : z3_a_val) : CrVal :=
+  match e with
+  | Z3Arith e' =>
+    eval_z3_arith e' sval aval
+  | Z3Ptr e' =>
+    eval_z3_ptr e' sval aval
+  | _ => ErrorVal
+  end.
+
+(* Check that bounds are equal for all variable arrays *)
+Definition query_bounds (p1 p2 : IM_Program) : bool_expr :=
+  let val1 := sym_eval_program p1 in
+  let val2 := sym_eval_program p2 in
+
+  (* Extract variable ids from input (uintptr_t) and output vaddrs *)
+  let input_vars := List.map fst (List.filter (fun '(_, t) => match t with uintptr_t => true | _ => false end) (fn_in p1)) in
+  let output_vars := List.map fst (fn_out_vaddrs p1) in
+  let bound_vars := input_vars ++ output_vars in
+
+  let b1 := List.map (vptr_bound val1) bound_vars in
+  let b2 := List.map (vptr_bound val2) bound_vars in
+  
+  fold_right Z3_Conj Z3_T
+    (map (fun '((_, x), (_, y)) => Z3_Eq x y) (combine b1 b2)).
+
+(* Check that outputs are equal (error flag, variables, and memory writes) *)
+Definition query_outputs (p1 p2 : IM_Program) : bool_expr :=
+  let val1 := sym_eval_program p1 in
+  let val2 := sym_eval_program p2 in
+
+  let o1 := (errored val1,
+             List.map (var_val val1) (fn_out_vars p1),
+             List.map (iptr_val val1) (fn_out_iaddrs p1),
+             List.map (vptr_val val1) (fn_out_vaddrs p1)) in
+  let o2 := (errored val2,
+             List.map (var_val val2) (fn_out_vars p2),
+             List.map (iptr_val val2) (fn_out_iaddrs p2),
+             List.map (vptr_val val2) (fn_out_vaddrs p2)) in
+  match o1, o2 with
+  | (e1, v1, ip1, vp1),
+    (e2, v2, ip2, vp2)  =>
+    let e_expr :=
+      if (orb (andb e1 e2) (andb (negb e1) (negb e2)))
+      then Z3_T
+      else Z3_F in
+    let v_expr := fold_right Z3_Conj Z3_T
+      (map (fun '((_, x), (_, y)) => Z3_Eq x y) (combine v1 v2)) in
+    let ip_expr := fold_right Z3_Conj Z3_T
+      (map (fun '((_, x), (_, y)) => Z3_Eq x y) (combine ip1 ip2)) in
+    let vp_expr := fold_right Z3_Conj Z3_T
+      (map (fun '((_, x), (_, y)) => Z3_Eq x y) (combine vp1 vp2)) in
+    Z3_Conj e_expr (
+    Z3_Conj v_expr (
+    Z3_Conj ip_expr
+            vp_expr))
+  end.
+
+(* Main query: check if outputs and bounds differ *)
+Definition query_expression (p1 p2 : IM_Program) : bool_expr :=
+  Z3_Neg (Z3_Conj (query_outputs p1 p2) (query_bounds p1 p2)).
+
+Inductive FailureMode :=
+| ValueMismatch
+| BoundsMismatch
+| FullMismatch.
+
+Inductive Z3Res :=
+| Z3Sat (s : z3_s_val) (a : z3_a_val) (f : FailureMode)
+| Z3Unsat
+| Z3Unknown.
+Parameter z3_query : bool_expr -> Z3Res.
+
+Axiom z3_sound_some:
+  forall e sval aval f,
+    z3_query e = Z3Sat sval aval f ->
+    eval_z3_bool e sval aval = true.
+Axiom z3_sound_none:
+  forall e,
+    z3_query e = Z3Unsat ->
+    forall sval aval,
+    eval_z3_bool e sval aval = false.
+
+Definition matching_fn_io (p1 p2 : IM_Program) : Prop :=
+  (fn_in p1) = (fn_in p2) /\
+  (fn_out_vars p1) = (fn_out_vars p2) /\
+  (fn_out_iaddrs p1) = (fn_out_iaddrs p2) /\
+  (fn_out_vaddrs p1) = (fn_out_vaddrs p2).
+
+Definition matching_error (p1 p2 : IM_Program) : Prop :=
+  forall (sval : z3_s_val) (aval : z3_a_val),
+    errored (sym_eval_program p1) = errored (sym_eval_program p2).
+Lemma mem_prog_soundness_error:
+  forall (p1 p2 : IM_Program),
+  matching_fn_io p1 p2 ->
+  z3_query (query_expression p1 p2) = Z3Unsat ->
+  matching_error p1 p2.
+Proof.
+  intros.
+Admitted.
+
+Definition matching_io_vars (p1 p2 : IM_Program) : Prop :=
+  forall (sval : z3_s_val) (aval : z3_a_val) (v : var_id),
+    In v (fn_out_vars p1) ->
+    eval_z3_expr
+      (snd ((var_val (sym_eval_program p1)) v))
+      sval aval =
+    eval_z3_expr
+      (snd ((var_val (sym_eval_program p2)) v))
+      sval aval.
+Lemma mem_prog_soundness_io_vars:
+  forall (p1 p2 : IM_Program),
+  matching_fn_io p1 p2 ->
+  z3_query (query_expression p1 p2) = Z3Unsat ->
+  matching_io_vars p1 p2.
+Proof.
+  intros.
+Admitted.
+
+Definition matching_abs_addrs (p1 p2 : IM_Program) : Prop :=
+  forall (sval : z3_s_val) (aval : z3_a_val) (ia : uintbptr) (ix1 : uint32),
+    In (ia, ix1) (fn_out_iaddrs p1) ->
+    eval_z3_expr
+      (snd ((iptr_val (sym_eval_program p1)) (ia, ix1)))
+      sval aval =
+    eval_z3_expr
+      (snd ((iptr_val (sym_eval_program p2)) (ia, ix1)))
+      sval aval.
+Lemma mem_prog_soundness_abs_addrs:
+  forall (p1 p2 : IM_Program),
+  matching_fn_io p1 p2 ->
+  z3_query (query_expression p1 p2) = Z3Unsat ->
+  matching_abs_addrs p1 p2.
+Proof.
+  intros.
+Admitted.
+
+Definition matching_var_addrs (p1 p2 : IM_Program) : Prop :=
+  forall (sval : z3_s_val) (aval : z3_a_val) (va : var_id) (ix2 : uint32),
+    In (va, ix2) (fn_out_vaddrs p1) ->
+    eval_z3_expr
+      (snd ((vptr_val (sym_eval_program p1)) (va, ix2)))
+      sval aval =
+    eval_z3_expr
+      (snd ((vptr_val (sym_eval_program p2)) (va, ix2)))
+      sval aval.
+Lemma mem_prog_soundness_var_addrs:
+  forall (p1 p2 : IM_Program),
+  matching_fn_io p1 p2 ->
+  z3_query (query_expression p1 p2) = Z3Unsat ->
+  matching_var_addrs p1 p2.
+Proof.
+  intros.
+Admitted.
+
+Definition matching_access_bounds (p1 p2 : IM_Program) : Prop :=
+  forall (sval : z3_s_val) (aval : z3_a_val) (va : var_id),
+    (In va (List.map fst (List.filter (fun '(_, t) => match t with uintptr_t => true | _ => false end) (fn_in p1))) \/
+     In va (List.map fst (fn_out_vaddrs p1))) ->
+    eval_z3_expr
+      (snd ((vptr_bound (sym_eval_program p1)) va))
+      sval aval =
+    eval_z3_expr
+      (snd ((vptr_bound (sym_eval_program p2)) va))
+      sval aval.
+Lemma mem_prog_soundness_access_bounds:
+  forall (p1 p2 : IM_Program),
+  matching_fn_io p1 p2 ->
+  z3_query (query_expression p1 p2) = Z3Unsat ->
+  matching_access_bounds p1 p2.
+Proof.
+  intros.
+Admitted.
+
+Lemma mem_prog_soundness:
+  forall (p1 p2 : IM_Program),
+  matching_fn_io p1 p2 ->
+  z3_query (query_expression p1 p2) = Z3Unsat ->
+    matching_error p1 p2 /\
+    matching_io_vars p1 p2 /\
+    matching_abs_addrs p1 p2 /\
+    matching_var_addrs p1 p2 /\
+    matching_access_bounds p1 p2.
+Proof with assumption.
+  intros. repeat split.
+  - apply mem_prog_soundness_error...
+  - apply mem_prog_soundness_io_vars...
+  - apply mem_prog_soundness_abs_addrs...
+  - apply mem_prog_soundness_var_addrs...
+  - apply mem_prog_soundness_access_bounds...
+Qed.
+
+Definition differing_error (p1 p2 : IM_Program) (sval : z3_s_val) (aval : z3_a_val) : Prop :=
+  errored (sym_eval_program p1) <> errored (sym_eval_program p2).
+
+Definition differing_io_vars (p1 p2 : IM_Program) (sval : z3_s_val) (aval : z3_a_val) : Prop :=
+  exists (v : var_id),
+    In v (fn_out_vars p1) /\
+    eval_z3_expr
+      (snd ((var_val (sym_eval_program p1)) v))
+      sval aval <>
+    eval_z3_expr
+      (snd ((var_val (sym_eval_program p2)) v))
+      sval aval.
+
+Definition differing_abs_addrs (p1 p2 : IM_Program) (sval : z3_s_val) (aval : z3_a_val) : Prop :=
+  exists (ia : uintbptr) (ix1 : uint32),
+    In (ia, ix1) (fn_out_iaddrs p1) /\
+    eval_z3_expr
+      (snd ((iptr_val (sym_eval_program p1)) (ia, ix1)))
+      sval aval <>
+    eval_z3_expr
+      (snd ((iptr_val (sym_eval_program p2)) (ia, ix1)))
+      sval aval.
+
+Definition differing_var_addrs (p1 p2 : IM_Program) (sval : z3_s_val) (aval : z3_a_val) : Prop :=
+  exists (va : var_id) (ix2 : uint32),
+    In (va, ix2) (fn_out_vaddrs p1) /\
+    eval_z3_expr
+      (snd ((vptr_val (sym_eval_program p1)) (va, ix2)))
+      sval aval <>
+    eval_z3_expr
+      (snd ((vptr_val (sym_eval_program p2)) (va, ix2)))
+      sval aval.
+
+Definition differing_access_bounds (p1 p2 : IM_Program) (sval : z3_s_val) (aval : z3_a_val) : Prop :=
+  exists (va : var_id),
+    (In va (List.map fst (List.filter (fun '(_, t) => match t with uintptr_t => true | _ => false end) (fn_in p1))) \/
+     In va (List.map fst (fn_out_vaddrs p1))) /\
+    eval_z3_expr
+      (snd ((vptr_bound (sym_eval_program p1)) va))
+      sval aval <>
+    eval_z3_expr
+      (snd ((vptr_bound (sym_eval_program p2)) va))
+      sval aval.
+
+Lemma mem_prog_completeness:
+  forall (p1 p2 : IM_Program) sval aval f,
+  matching_fn_io p1 p2 ->
+  z3_query (query_expression p1 p2) = Z3Sat sval aval f ->
+  differing_error p1 p2 sval aval \/
+  differing_io_vars p1 p2 sval aval \/
+  differing_abs_addrs p1 p2 sval aval \/
+  differing_var_addrs p1 p2 sval aval \/
+  differing_access_bounds p1 p2 sval aval.
+Proof.
+  intros.
+Admitted.
