CrMemEx.v
@@ -1,0 +1,246 @@
+From MyProject Require Import CrMem.
+From MyProject Require Import CrVal.
+From MyProject Require Import CrIdentifiers.
+From MyProject Require Import SmtExpr.
+From MyProject Require Import Maps.
+From MyProject Require Import Integers.
+From MyProject Require Import MyInts.
+Require Import ZArith.
+From Coq.Strings Require Import String.
+From Coq.Strings Require Import Ascii.
+Require Import List.
+Import ListNotations.
+
+
+Definition rdi : positive := 1.
+Definition rsi : positive := 2.
+Definition rdx : positive := 3.
+Definition rcx : positive := 4.
+Definition rax : positive := 5.
+
+Definition local_x := (TmpArg 1%positive).
+Definition b_plus_c := (TmpArg 2%positive).
+Definition x4_val := (TmpArg 3%positive).
+Definition two_plus_two := (TmpArg 4%positive).
+
+Definition p1a : IM_Program := {|
+  fn_in := [
+    (rdi, uintptr_t);
+    (rsi, uint8_t);
+    (rdx, uint8_t)
+  ];
+  fn_body := [
+    AllocOp local_x
+      (ValArg (imm_ptr (repr 0x400)))
+      (ValArg (imm_u32 (repr 16)));
+    Binary AddOp b_plus_c
+      (IOArg rsi)
+      (IOArg rdx);
+    StOp local_x
+      (ValArg (imm_u32 (repr 4)))
+      b_plus_c;
+    LdOp x4_val
+      local_x
+      (ValArg (imm_u32 (repr 4)));
+    StOp (IOArg rdi)
+      (ValArg (imm_u32 (repr 0)))
+      x4_val
+  ];
+  fn_out_vars := [];
+  fn_out_iaddrs := [];
+  fn_out_vaddrs := [(rdi, (repr 0))];
+|}.
+
+(* Compute List.map (vptr_val (compile_sym p1)) (fn_out_vaddrs p1). *)
+
+Definition p1b : IM_Program := {|
+  fn_in := [
+    (rdi, uintptr_t);
+    (rsi, uint8_t);
+    (rdx, uint8_t)
+  ];
+  fn_body := [
+    AllocOp local_x
+      (ValArg (imm_ptr (repr 0x400)))
+      (ValArg (imm_u32 (repr 16)));
+    Binary AddOp b_plus_c
+      (IOArg rsi)
+      (IOArg rdx);
+    Binary AddOp two_plus_two
+      (ValArg (imm_u32 (repr 2)))
+      (ValArg (imm_u32 (repr 2)));
+    StOp local_x
+      (ValArg (imm_u32 (repr 4)))
+      b_plus_c;
+    LdOp x4_val
+      local_x
+      two_plus_two;
+    StOp (IOArg rdi)
+      (ValArg (imm_u32 (repr 0)))
+      x4_val
+  ];
+  fn_out_vars := [];
+  fn_out_iaddrs := [];
+  fn_out_vaddrs := [(rdi, (repr 0))];
+|}.
+
+Definition p1c : IM_Program := {|
+  fn_in := [
+    (rdi, uintptr_t);
+    (rsi, uint8_t);
+    (rdx, uint8_t)
+  ];
+  fn_body := [
+    AllocOp local_x
+      (ValArg (imm_ptr (repr 0x400)))
+      (ValArg (imm_u32 (repr 16)));
+    Binary AddOp b_plus_c
+      (IOArg rsi)
+      (IOArg rdx);
+    StOp local_x
+      (ValArg (imm_u32 (repr 4)))
+      b_plus_c;
+    LdOp x4_val
+      local_x
+      (ValArg (imm_u32 (repr 4)));
+    StOp (IOArg rdi)
+      (ValArg (imm_u32 (repr 0)))
+      x4_val;
+    StOp (IOArg rdi)
+      (ValArg (imm_u32 (repr 0)))
+      (ValArg (imm_u8 (repr 1)))
+  ];
+  fn_out_vars := [];
+  fn_out_iaddrs := [];
+  fn_out_vaddrs := [(rdi, (repr 0))];
+|}.
+
+Definition p2a : IM_Program := {|
+  fn_in := [
+    (rdi, uintptr_t);
+    (rax, uint8_t)
+  ];
+  fn_body := [
+    LdOp (IOArg rax)
+      (IOArg rdi)
+      (ValArg (imm_u32 (repr 0)))
+  ];
+  fn_out_vars := [rax];
+  fn_out_iaddrs := [];
+  fn_out_vaddrs := [];
+|}.
+Definition p2b : IM_Program := {|
+  fn_in := [
+    (rdi, uintptr_t);
+    (rax, uint8_t)
+  ];
+  fn_body := [
+    LdOp (TmpArg 1%positive)
+      (IOArg rdi)
+      (ValArg (imm_u32 (repr 1)));
+    LdOp (IOArg rax)
+      (IOArg rdi)
+      (ValArg (imm_u32 (repr 0)))
+  ];
+  fn_out_vars := [rax];
+  fn_out_iaddrs := [];
+  fn_out_vaddrs := [];
+|}.
+Definition p2c : IM_Program := {|
+  fn_in := [
+    (rdi, uintptr_t);
+    (rax, uint8_t)
+  ];
+  fn_body := [
+    LdOp (IOArg rax)
+      (IOArg rdi)
+      (ValArg (imm_u32 (repr 0)));
+    StOp (IOArg rdi)
+      (ValArg (imm_u32 (repr 1)))
+      (ValArg (imm_u8 (repr 0)))
+  ];
+  fn_out_vars := [rax];
+  fn_out_iaddrs := [];
+  fn_out_vaddrs := [];
+|}.
+
+Definition p3a : IM_Program := {|
+  fn_in := [
+    (rdi, uint8_t);
+    (rsi, uintptr_t);
+    (rax, uint8_t)
+  ];
+  fn_body := [
+    BrzOp (ValArg (imm_u8 (repr 0)))
+      [
+        Binary AddOp (IOArg rax)
+          (IOArg rdi)
+          (ValArg (imm_u8 (repr 0)))
+      ]
+      [
+        LdOp (IOArg rax)
+          (IOArg rsi)
+          (ValArg (imm_u32 (repr 0)))
+      ]
+  ];
+  fn_out_vars := [rax];
+  fn_out_iaddrs := [];
+  fn_out_vaddrs := [];
+|}.
+Definition p3b : IM_Program := {|
+  fn_in := [
+    (rdi, uint8_t);
+    (rsi, uintptr_t);
+    (rax, uint8_t)
+  ];
+  fn_body := [
+    Binary AddOp (IOArg rax)
+      (IOArg rdi)
+      (ValArg (imm_u8 (repr 0)))
+  ];
+  fn_out_vars := [rax];
+  fn_out_iaddrs := [];
+  fn_out_vaddrs := [];
+|}.
+
+Definition p4a : IM_Program := {|
+  fn_in := [
+    (rdi, uintptr_t);
+    (rax, uint8_t)
+  ];
+  fn_body := [
+    LdOp (IOArg rax)
+      (IOArg rdi)
+      (ValArg (imm_u32 (repr 1)));
+    LdOp (IOArg rax)
+      (IOArg rdi)
+      (ValArg (imm_u32 (repr 0)))
+  ];
+  fn_out_vars := [rax];
+  fn_out_iaddrs := [];
+  fn_out_vaddrs := [];
+|}.
+Definition p4b : IM_Program := {|
+  fn_in := [
+    (rdi, uintptr_t);
+    (rax, uint8_t)
+  ];
+  fn_body := [
+    LdOp (IOArg rax)
+      (IOArg rdi)
+      (ValArg (imm_u32 (repr 0)));
+    LdOp (IOArg rax)
+      (IOArg rdi)
+      (ValArg (imm_u32 (repr 1)))
+  ];
+  fn_out_vars := [rax];
+  fn_out_iaddrs := [];
+  fn_out_vaddrs := [];
+|}.
+
+Definition example_programs := [
+  p1a; p1b; p1c;
+  p2a; p2b; p2c;
+  p3a; p3b;
+  p4a; p4b
+].
