CrVal.v
@@ -1,0 +1,278 @@
+Require Import ZArith.
+From MyProject Require Import MyInts.
+From MyProject Require Import Integers.
+From MyProject Require Import Maps.
+
+Inductive Check_T (T : Type) :=
+| Legal (v : T)
+| Illegal.
+Arguments Legal {T} _.
+Arguments Illegal {T}.
+
+Inductive CrInt_T : Type :=
+| CrUInt8 (val : uint8)
+| CrUInt16 (val : uint16)
+| CrUInt32 (val : uint32)
+| CrUInt64 (val : uint64)
+| CrNilInt.
+Inductive CrPtr_T : Type :=
+| CrPtr (addr : uintbptr)
+| CrNilPtr.
+Inductive CrVal : Type :=
+| IntVal (val : CrInt_T)
+| PtrVal (val : CrPtr_T)
+| UninitVal
+| ErrorVal.
+
+Inductive MemVal (T : Type) :=
+| Init (v : T)
+| Uninit.
+Arguments Init {T} _.
+Arguments Uninit {T}.
+Record MemBlock (T : Type) := {
+  arr_len : uint32;
+  arr_bytes : PMap.t (MemVal T);
+}.
+Arguments arr_len {T} _.
+Arguments arr_bytes {T} _.
+Inductive Array {T : Type} :=
+| Allocated (arr : MemBlock T)
+| Unallocated.
+Arguments Unallocated {T}.
+Inductive Memory (T : Type) :=
+| Mem (m : PMap.t (@Array T))
+| Invalid.
+Arguments Mem {T} _.
+Arguments Invalid {T}.
+
+(* requires S to prevent collision @ 0 *)
+Definition pkey_to_mkey {w} (p : @bit_int w) : positive :=
+  Pos.of_nat (S (Z.to_nat (unsigned p))).
+
+Definition iveqb (x y : CrInt_T) : bool :=
+  match x, y with
+  | CrUInt8 x', CrUInt8 y'
+  | CrUInt16 x', CrUInt16 y'
+  | CrUInt32 x', CrUInt32 y'
+  | CrUInt64 x', CrUInt64 y' => Integers.eq x' y'
+  | CrNilInt, CrNilInt => true
+  | _, _ => false
+  end.
+Transparent iveqb.
+Definition eqb (x y : CrVal) : bool :=
+  match x, y with
+  | IntVal x', IntVal y' => iveqb x' y'
+  | PtrVal (CrPtr x'), PtrVal (CrPtr y') => Integers.eq x' y'
+  | PtrVal (CrNilPtr), PtrVal (CrNilPtr) => true
+  | UninitVal, UninitVal
+  | ErrorVal, ErrorVal => true
+  | _, _ => false
+  end.
+
+Definition ivltb (x y : CrInt_T) : bool :=
+  match x, y with
+  | CrUInt8 x', CrUInt8 y'
+  | CrUInt16 x', CrUInt16 y'
+  | CrUInt32 x', CrUInt32 y'
+  | CrUInt64 x', CrUInt64 y' => Integers.lt x' y'
+  | _, _ => false
+  end.
+Transparent ivltb.
+Definition ltb (x y : CrVal) : bool :=
+  match x, y with
+  | IntVal x', IntVal y'
+    => ivltb x' y'
+  | PtrVal (CrPtr x'), PtrVal (CrPtr y')
+    => Integers.lt x' y'
+  | _, _ => false
+  end.
+
+Definition apply_iv_binop
+  (f :forall (w : positive), @bit_int w -> @bit_int w -> @bit_int w)
+  (x y : CrInt_T) : CrVal :=
+  match x, y with
+  | CrUInt8 x', CrUInt8 y'
+    => IntVal (CrUInt8 (@f _ x' y'))
+  | CrUInt16 x', CrUInt16 y'
+    => IntVal (CrUInt16 (@f _ x' y'))
+  | CrUInt32 x', CrUInt32 y'
+    => IntVal (CrUInt32 (@f _ x' y'))
+  | CrUInt64 x', CrUInt64 y'
+    => IntVal (CrUInt64 (@f _ x' y'))
+  | _, _ => ErrorVal
+  end.
+Transparent apply_iv_binop.
+
+Definition add (x y : CrVal) : CrVal :=
+  match x, y with
+  | IntVal x', IntVal y' => apply_iv_binop (fun w => @Integers.add w) x' y'
+  | _, _ => ErrorVal
+  end.
+
+Definition sub (x y : CrVal) : CrVal :=
+  match x, y with
+  | IntVal x', IntVal y' => apply_iv_binop (fun w => @Integers.sub w) x' y'
+  | _, _ => ErrorVal
+  end.
+
+Definition and (x y : CrVal) : CrVal :=
+  match x, y with
+  | IntVal x', IntVal y' => apply_iv_binop (fun w => @Integers.and w) x' y'
+  | _, _ => ErrorVal
+  end.
+
+Definition or (x y : CrVal) : CrVal :=
+  match x, y with
+  | IntVal x', IntVal y' => apply_iv_binop (fun w => @Integers.or w) x' y'
+  | _, _ => ErrorVal
+  end.
+
+Definition xor (x y : CrVal) : CrVal :=
+  match x, y with
+  | IntVal x', IntVal y' => apply_iv_binop (fun w => @Integers.xor w) x' y'
+  | _, _ => ErrorVal
+  end.
+
+Definition not (x : CrVal) : CrVal :=
+  match x with
+  | IntVal (CrUInt8 x')
+    => IntVal (CrUInt8 (Integers.not x'))
+  | IntVal (CrUInt16 x')
+    => IntVal (CrUInt16 (Integers.not x'))
+  | IntVal (CrUInt32 x')
+    => IntVal (CrUInt32 (Integers.not x'))
+  | IntVal (CrUInt64 x')
+    => IntVal (CrUInt64 (Integers.not x'))
+  | _ => ErrorVal
+  end.
+
+Definition mul (x y : CrVal) : CrVal :=
+  match x, y with
+  | IntVal x', IntVal y' => apply_iv_binop (fun w => @Integers.mul w) x' y'
+  | _, _ => ErrorVal
+  end.
+
+Definition divu (x y : CrVal) : CrVal :=
+  match x, y with
+  | IntVal x', IntVal y' => apply_iv_binop (fun w => @Integers.divu w) x' y'
+  | _, _ => ErrorVal
+  end.
+
+Definition modu (x y : CrVal) : CrVal :=
+  match x, y with
+  | IntVal x', IntVal y' => apply_iv_binop (fun w => @Integers.modu w) x' y'
+  | _, _ => ErrorVal
+  end.
+
+Definition ld_arr (a : Array) (i : CrVal) : Check_T CrVal :=
+  match a, i with
+  | Allocated array, IntVal (CrUInt32 idx) =>
+    if (Integers.ltu idx (arr_len array)) then
+      match (arr_bytes array) !! (pkey_to_mkey idx) with
+      | Init v => Legal v
+      | Uninit => Legal UninitVal
+      end
+    else
+      Illegal
+  | _, _ => Illegal
+  end.
+
+Definition ld (m : Memory CrVal) (p : CrVal) (i : CrVal) : Check_T CrVal :=
+  match m with
+  | Mem m' =>
+    match p with
+    | PtrVal (CrPtr addr) =>
+      ld_arr (m' !! (pkey_to_mkey addr)) i
+    | _ => Illegal
+    end 
+  | Invalid => Illegal
+  end.
+
+Definition st_arr (a : Array) (i : CrVal) (v : CrVal) : Check_T Array :=
+  match a, i with
+  | Allocated array, IntVal (CrUInt32 idx) =>
+    if (Integers.ltu idx (arr_len array)) then
+      Legal (Allocated {|
+        arr_len := arr_len array;
+        arr_bytes := PMap.set (pkey_to_mkey idx) (Init v) (arr_bytes array);
+      |})
+    else
+      Illegal
+  | _, _ => Illegal
+  end.
+
+Definition st (m : Memory CrVal) (p : CrVal) (i : CrVal) (v : CrVal) : Memory CrVal :=
+  match m with
+  | Mem m' =>
+    match p with
+    | PtrVal (CrPtr addr) =>
+      match st_arr (m' !! (pkey_to_mkey addr)) i v with
+      | Legal arr => Mem (PMap.set (pkey_to_mkey addr) arr m')
+      | Illegal => Invalid
+      end
+    | _ => Invalid
+    end
+  | Invalid => Invalid
+  end.
+
+Definition tabula_rasa {T : Type} : Memory T :=
+  Mem (PMap.init Unallocated).
+
+(* TODO: Handle allocation collisions i.e. set mem to Invalid *)
+Definition alloc {T : Type} (m : Memory T) (arg1 : CrVal) (arg2 : CrVal) : Memory T :=
+  match m with
+  | Mem m' =>
+    match arg1, arg2 with
+    | PtrVal (CrPtr addr), IntVal (CrUInt32 idx) => Mem
+        (PMap.set (pkey_to_mkey addr) (Allocated {|
+          arr_len := idx;
+          arr_bytes := PMap.init Uninit;
+      |}) m')
+    | _, _ => Invalid
+    end
+  | Invalid => Invalid
+  end.
+
+(* TODO: Handle double free *)
+Definition free {T : Type} (m : Memory T) (arg1 : CrVal) : Memory T :=
+  match m with
+  | Mem m' =>
+    match arg1 with
+    | PtrVal (CrPtr b) => Mem
+        (PMap.set (pkey_to_mkey b) Unallocated m')
+    | _ => Invalid
+    end
+  | Invalid => Invalid
+  end.
+
+Lemma crval_concrete_if_else : forall (v1 v2 : CrVal),
+  ((if eqb v1 v2 then true else false) = true)->
+  v1 = v2.
+Proof.
+  intros v1 v2 H.
+  unfold eqb, eq, Rocqlib.zeq in H.
+  destruct v1, v2; try reflexivity; try discriminate;
+  try (destruct val; exfalso; congruence);
+  destruct val; destruct val0; try discriminate; try reflexivity; simpl in *; unfold eq in *;
+  try destruct (BinInt.Z.eq_dec (unsigned val) (unsigned val0)); try discriminate;
+  try destruct (BinInt.Z.eq_dec (unsigned addr) (unsigned addr0)); try discriminate;
+  try apply uintw_eq_from_unsigned in e; try rewrite e; try reflexivity;
+  destruct (Rocqlib.zeq (unsigned val) (unsigned val0)); try congruence.
+Qed.
+
+Lemma crval_concrete_if_else2 : forall (v1 v2 : CrVal),
+  ((if eqb v1 v2 then true else false) = false)->
+  v1 <> v2.
+Proof.
+  intros v1 v2 H.
+  destruct v1, v2; try discriminate;
+  unfold eqb in H;
+  unfold iveqb in H;
+  unfold eq in H;
+  unfold Rocqlib.zeq in H;
+  injection;
+  destruct val, val0; try congruence;
+  try destruct (BinInt.Z.eq_dec (unsigned val) (unsigned val0)); try discriminate;
+  try destruct (BinInt.Z.eq_dec (unsigned addr) (unsigned addr0)); try discriminate;
+  apply uintw_neq_from_unsigned in n; congruence.
+Qed.
