SmtExpr.v
@@ -1,10 +1,12 @@
 (* Write out semantics for bitvectors in SMT,
-   show that a single hdr_op evaluation can be converted to the appropriate SMT formula in Z3 *)
+show that a single hdr_op evaluation can be converted to the appropriate SMT formula in Z3 *)
 From MyProject Require Import CrIdentifiers.
 From MyProject Require Import MyInts.
 From MyProject Require Import SmtTypes.
+From MyProject Require Import CrVal.
 From Coq.Strings Require Import String.
 
+(* TODO: Look through K2 code *)
 Inductive SmtBoolExpr : Type :=
     | SmtTrue
     | SmtFalse
@@ -13,7 +15,7 @@ Inductive SmtBoolExpr : Type :=
     | SmtBoolOr (e1 e2 : SmtBoolExpr)
     | SmtBoolEq (e1 e2 : SmtArithExpr)
 with SmtArithExpr : Type :=
-    | SmtConst (value : uint8)
+    | SmtArithConst (value : CrInt_T)
     | SmtArithVar (name : string)
     | SmtConditional (cond : SmtBoolExpr) (then_expr else_expr : SmtArithExpr)
     (* Arithmetic operations *)
@@ -26,7 +28,14 @@ with SmtArithExpr : Type :=
     | SmtBitNot (e : SmtArithExpr)
     | SmtBitMul (e1 e2 : SmtArithExpr)
     | SmtBitDiv (e1 e2 : SmtArithExpr)
-    | SmtBitMod (e1 e2 : SmtArithExpr).
+    | SmtBitMod (e1 e2 : SmtArithExpr)
+    | SmtArrSel (e1 : SmtArrExpr) (e2 : (*SmtPtrExpr*) SmtArithExpr) (e3 : SmtArithExpr)
+(* with SmtPtrExpr : Type := *)
+    | SmtPtrConst (e1 : CrPtr_T) (* e.g. 0x7fffffff0000 *)
+    | SmtPtrVar (e1 : string) (* e.g. x *)
+with SmtArrExpr : Type :=
+    | SmtArrInit
+    | SmtArrSt (e1 : SmtArrExpr) (e2 : (*SmtPtrExpr*) SmtArithExpr) (e3 : SmtArithExpr) (e4 : SmtArithExpr).
 
 (* Evaluate a SMT Bool expression given a valuation *)
 Fixpoint eval_smt_bool (e : SmtBoolExpr) (v : SmtValuation) : bool :=
@@ -36,24 +45,73 @@ Fixpoint eval_smt_bool (e : SmtBoolExpr) (v : SmtValuation) : bool :=
     | SmtBoolNot e' => negb (eval_smt_bool e' v)
     | SmtBoolAnd e1 e2 => andb (eval_smt_bool e1 v) (eval_smt_bool e2 v)
     | SmtBoolOr e1 e2 => orb (eval_smt_bool e1 v) (eval_smt_bool e2 v)
-    | SmtBoolEq e1 e2 => if (Integers.eq (eval_smt_arith e1 v) (eval_smt_arith e2 v)) then true else false
+    | SmtBoolEq e1 e2 => if (CrVal.eqb
+      (eval_smt_arith e1 v) (eval_smt_arith e2 v)) then true else false
     end
-with eval_smt_arith (e : SmtArithExpr) (v : SmtValuation) : uint8 :=
+with eval_smt_arith (e : SmtArithExpr) (v : SmtValuation) : CrVal :=
     match e with
-    | SmtConst value => value
-    | SmtArithVar name => v name
-    | SmtConditional cond then_expr else_expr => 
+    | SmtArithConst value => IntVal value
+    | SmtArithVar name => match v name with
+      | IntVal v' => IntVal v'
+      | _ => ErrorVal
+      end
+    | SmtConditional cond then_expr else_expr =>
         if eval_smt_bool cond v 
-        then eval_smt_arith then_expr v 
-        else eval_smt_arith else_expr v
-    | SmtBitAdd e1 e2 => Integers.add (eval_smt_arith e1 v) (eval_smt_arith e2 v)
-    | SmtBitSub e1 e2 => Integers.sub (eval_smt_arith e1 v) (eval_smt_arith e2 v)
-    | SmtBitAnd e1 e2 => Integers.and (eval_smt_arith e1 v) (eval_smt_arith e2 v)
-    | SmtBitOr e1 e2 =>  Integers.or (eval_smt_arith e1 v) (eval_smt_arith e2 v)
-    | SmtBitXor e1 e2 => Integers.xor (eval_smt_arith e1 v) (eval_smt_arith e2 v)
-    | SmtBitNot e =>     Integers.not (eval_smt_arith e v)
-    | SmtBitMul e1 e2 => Integers.mul (eval_smt_arith e1 v) (eval_smt_arith e2 v)
-    | SmtBitDiv e1 e2 => Integers.divu (eval_smt_arith e1 v) (eval_smt_arith e2 v)
-    | SmtBitMod e1 e2 => Integers.modu (eval_smt_arith e1 v) (eval_smt_arith e2 v)
+        then (eval_smt_arith then_expr v)
+        else (eval_smt_arith else_expr v)
+    | SmtBitAdd e1 e2 => CrVal.add
+        (eval_smt_arith e1 v)
+        (eval_smt_arith e2 v)
+    | SmtBitSub e1 e2 => CrVal.sub
+        (eval_smt_arith e1 v)
+        (eval_smt_arith e2 v)
+    | SmtBitAnd e1 e2 => CrVal.and
+        (eval_smt_arith e1 v)
+        (eval_smt_arith e2 v)
+    | SmtBitOr e1 e2 => CrVal.or
+        (eval_smt_arith e1 v)
+        (eval_smt_arith e2 v)
+    | SmtBitXor e1 e2 => CrVal.xor
+        (eval_smt_arith e1 v)
+        (eval_smt_arith e2 v)
+    | SmtBitNot e => CrVal.not (eval_smt_arith e v)
+    | SmtBitMul e1 e2 => CrVal.mul
+        (eval_smt_arith e1 v)
+        (eval_smt_arith e2 v)
+    | SmtBitDiv e1 e2 => CrVal.divu
+        (eval_smt_arith e1 v)
+        (eval_smt_arith e2 v)
+    | SmtBitMod e1 e2 => CrVal.modu
+        (eval_smt_arith e1 v)
+        (eval_smt_arith e2 v)
+    | SmtArrSel e1 e2 e3 =>
+        match CrVal.ld
+            (eval_smt_mem e1 v)
+            (eval_smt_arith e2 v)
+            (eval_smt_arith e3 v)
+        with
+        | Legal v' => v'
+        | Illegal => ErrorVal
+        end
+    | SmtPtrConst value => PtrVal value
+    | SmtPtrVar name => match v name with
+      | PtrVal v' => PtrVal v'
+      | _ => ErrorVal
+      end
+    end
+(* with eval_smt_ptr (e : SmtPtrExpr) (v : SmtValuation) : CrVal :=
+    unwrap_val match e with
+    | SmtPtrConst value => Legal (PtrVal value)
+    | SmtPtrVar name => match v name with
+      | PtrVal v' => Legal (PtrVal v')
+      | _ => Illegal
+      end
+    | SmtPtrAdd e1 e2 => CrVal.add (eval_smt_ptr e1 v) (eval_smt_arith e2 v)
+    end *)
+with eval_smt_mem (e : SmtArrExpr) (v : SmtValuation) : Memory CrVal :=
+    match e with
+    | SmtArrInit => @CrVal.tabula_rasa CrVal
+    | SmtArrSt e1 e2 e3 e4 => CrVal.st (eval_smt_mem e1 v) ((*eval_smt_ptr*) eval_smt_arith e2 v) (eval_smt_arith e3 v) (eval_smt_arith e4 v)
     end.
+
 (* InitStatus: might be unnecessary and error prone because Z3 may not map 1-to-1 to this. *)
